proof/correctness/Repr2.ec
@@ -6,15 +6,32 @@ from Jasmin require import JModel.
 
 (*****) import StdBigop.Bigint.
 
-require import Params Types WOTS XMSS_Params XMSS_MT_Types.
+require import Params Parameters Types WOTS XMSS_MT_Params LTree XMSS_MT_Types.
 
 require import Array32 Array64 Array68 Array132 Array136 Array2144.
 
 require import BitEncoding.
 (*---*) import BitChunking.
 
+require import Utils2.
+
+
 (* Encode : impl -> spec *)
 (* Decode : spec -> impl *)
+
+(** -------------------------------------------------------------------------------------------- **)
+
+op sub_list ['a] (x : 'a list) (k len : int) : 'a list = 
+  mkseq (fun (i : int) => nth witness x (k + i)) len.
+
+lemma size_sub_list (x : 'a list) (k len : int) :
+    0 <= len =>
+      size (sub_list x k len) = len.
+proof.
+move => ?.
+rewrite /sub_list size_mkseq /#.
+qed.
+
 
 (** -------------------------------------------------------------------------------------------- **)
 
@@ -102,13 +119,27 @@ op DecodeWotsSk (sk : wots_sk) : W8.t Array2144.t =
 op DecodeWotsPk (pk : wots_pk) : W8.t Array2144.t = 
   Array2144.of_list witness (nbytes_flatten (val pk)).
 
+op EncodeWotsSignature (s : W8.t Array2144.t) : wots_signature = 
+  LenNBytes.insubd (map NBytes.insubd (chunk 32 (to_list s))). 
+
+op EncodeWotsSignatureList (s : W8.t list) : wots_signature = 
+  LenNBytes.insubd (map NBytes.insubd (chunk 32 s)). 
+
 (** -------------------------------------------------------------------------------------------- **)
 
-lemma wots_sk_size (sk : wots_sk) : size (val sk) = len by smt(LenNBytes.valP).
-
-lemma wotS_sk_ssize (sk : wots_sk) :
+lemma wots_sk_ssize (sk : wots_sk) :
     forall (t : nbytes), t \in val sk => size (val t) = n
       by smt(NBytes.valP).
+
+lemma wots_sig_size_flatten (s : wots_signature) :
+    n = 32 /\ len = 67 =>
+    size (flatten (map NBytes.val (val s))) = 2144.
+proof.
+move => [#] n_val len_val.
+rewrite size_flatten sumzE BIA.big_map /(\o) //=. 
+rewrite -(StdBigop.Bigint.BIA.eq_big_seq (fun _ => 32)) 1:#smt:(wots_sk_ssize @List @NBytes).
+by rewrite big_constz count_predT size_map valP len_val.
+qed.
 
 (** -------------------------------------------------------------------------------------------- **)
 
@@ -118,10 +149,43 @@ op DecodePk (x : xmss_pk) : W8.t Array68.t =
 op DecodePkNoOID (x : xmss_pk) : W8.t Array64.t = 
   Array64.of_list witness (val x.`pk_root ++ val x.`pk_pub_seed).
 
+op EncodePk (x : W8.t Array68.t) : xmss_pk = {| pk_oid      = W32ofBytes (sub x 0 4);
+                                                pk_root     = NBytes.insubd (sub x 4 32); 
+                                                pk_pub_seed = NBytes.insubd (sub x 36 32); 
+                                              |}.
+
+op EncodePkNoOID (x : W8.t Array64.t) : xmss_pk = {| pk_oid      = witness;
+                                                     pk_root     = NBytes.insubd (sub x 0 32); 
+                                                     pk_pub_seed = NBytes.insubd (sub x 32 32);
+                                                   |}. 
+
 op DecodeSk (x : xmss_sk) : W8.t Array136.t = 
   Array136.of_list witness (W32toBytes impl_oid ++ W32toBytes x.`idx ++ val x.`sk_seed ++ 
                             val x.`sk_prf ++ val x.`sk_root ++ val x.`pub_seed_sk).
 
 op DecodeSkNoOID (x : xmss_sk) : W8.t Array132.t = 
-  Array132.of_list witness (W32toBytes x.`idx ++ val x.`sk_seed ++ val x.`sk_prf ++ val x.`sk_root ++ val  x.`pub_seed_sk).
+  Array132.of_list witness (W32toBytes x.`idx ++ val x.`sk_seed ++ val x.`sk_prf ++ 
+                            val x.`sk_root ++ val  x.`pub_seed_sk).
 
+(** -------------------------------------------------------------------------------------------- **)
+
+(* FIXME: Does this work for d > 1? *)
+op EncodeAuthPath (x : W8.t list) : auth_path = 
+  AuthPath.insubd [NBytes.insubd (sub_list x 0 32)].
+
+op EncodeReducedSignature (x : W8.t list) :  wots_signature * auth_path =
+  (EncodeWotsSignatureList (sub_list x 0 2144), EncodeAuthPath (sub_list x 2144 32)).
+
+(* sm = m || sig 
+   we use mlen to skip the m part
+
+   we receive a ptr to the signed message (= m || sig) and skip the m part
+*)
+op load_signature_mem (mem : global_mem_t) (sm_ptr mlen : W64.t) : W8.t list = 
+  mkseq (fun (i : int) => loadW8 mem (to_uint (sm_ptr + mlen) + i)) XMSS_SIG_BYTES.
+
+op EncodeSignature (sig_bytes : W8.t list) : sig_t =
+  {| sig_idx  = W32ofBytes (sub_list sig_bytes 0 4);
+     r        = NBytes.insubd (sub_list sig_bytes 4 32);
+     r_sigs   = map EncodeReducedSignature (chunk 2176 (sub_list sig_bytes 36 (36 - 2500)));
+  |}.
