proof/correctness/VerifyProof.ec
@@ -1,0 +1,523 @@
+pragma Goals : printall.
+
+require import AllCore List RealExp IntDiv Distr DList IntDiv.
+from Jasmin require import JModel JArray.
+
+require import Params Types Address Hash XMSS_MT_Params XMSS_MT_TreeHash XMSS_MT_Types XMSS_MT_PRF.
+require import XMSS_IMPL Parameters.
+
+require import Repr2 Utils2.
+
+require import Array4 Array8 Array32 Array64 Array68 Array96 Array132 Array136 Array352 Array2144.
+require import WArray32 WArray96 WArray136.
+
+require import Correctness_Address Correctness_Mem Correctness_Hash.
+require import DistrUtils.
+
+require import BitEncoding.
+(*---*) import BitChunking.
+
+require import StdBigop. 
+(*---*) import Bigint.
+
+require import Termination.
+
+lemma load_store_W64 (mem : global_mem_t) (a : address) (v : W64.t) :
+    loadW64 (storeW64 mem a v) a = v.
+proof.
+rewrite /loadW64 /storeW64 wordP => j?.
+rewrite pack8E /stores initiE // => />. 
+rewrite initiE 1:/# => />. 
+rewrite get_setE.
+  + case (a + j %/ 8 = a + 7) => *; [rewrite /(\bits8) initiE /# |].
+rewrite get_setE.
+  + case (a + j %/ 8 = a + 6) => *; [rewrite /(\bits8) initiE /# |].
+rewrite get_setE.
+  + case (a + j %/ 8 = a + 5) => *; [rewrite /(\bits8) initiE /# |].
+rewrite get_setE.
+  + case (a + j %/ 8 = a + 4) => *; [rewrite /(\bits8) initiE /# |].
+rewrite get_setE.
+  + case (a + j %/ 8 = a + 3) => *; [rewrite /(\bits8) initiE /# |].
+rewrite get_setE.
+  + case (a + j %/ 8 = a + 2) => *; [rewrite /(\bits8) initiE /# |].
+rewrite get_setE.
+  + case (a + j %/ 8 = a + 1) => *; [rewrite /(\bits8) initiE /# |].
+rewrite get_setE.
+  + rewrite ifT 1:/# /(\bits8) initiE /#.
+qed.
+
+lemma set_result_post (eq : W8.t) :
+    hoare[
+      M(Syscall).__set_result :
+      arg.`1 = eq
+      ==>
+      (eq = W8.zero) => res = W64.zero /\
+      (eq <> W8.zero) => res = W64.of_int (-1)
+    ].
+proof.
+proc.
+auto => />.
+case (eq = W8.zero). 
+  + rcondf 1; first by skip => [#] ?? => /#.
+    call (: true ==> true); last by auto.
+    proc; inline; wp; sp; while (true); auto => />. 
+  + rcondt 1; first by skip => [#] ?? => /#. 
+    auto => />. 
+qed.
+
+
+lemma p_set_result_post (eq : W8.t) :
+    phoare[
+      M(Syscall).__set_result :
+      arg.`1 = eq
+      ==>
+      (eq = W8.zero) => res = W64.zero /\
+      (eq <> W8.zero) => res = W64.of_int (-1)
+    ] = 1%r.
+proof.
+conseq set_result_ll (set_result_post eq).
+  + admit. (* Need to add stuff to #pre *)
+  + admit.
+qed.
+
+(*
+
+arg{1}
+
+m_ptr : W64.t         => ptr to the message 
+mlen_ptr : W64.t      => ptr to the message length 
+sm_ptr : W64.t        => ptr to the signed message
+smlen : W64.t         => length of the signed message = mlen + sig bytes
+pk : W8.t Array64.t   => public key
+
+arg{2}
+
+pk : xmss_pk  => public key 
+m : msg_t     => message 
+s : sig_t    => signature How to encode signature ?
+*)
+
+(* Load the signed message from memory. res = m || sig *)
+op load_sm_mem (mem : global_mem_t) (ptr sm_len : W64.t) : W8.t list =
+    mkseq (fun (i : int) => loadW8 mem (to_uint ptr + i)) (to_uint sm_len).
+
+(* Load the signature from memory. Skips the message *)
+op load_sig_mem (mem : global_mem_t) (sm_ptr sm_len : W64.t) : W8.t list =
+    let mlen : int = to_uint sm_len - XMSS_SIG_BYTES in
+    mkseq (fun (i : int) => loadW8 mem (to_uint sm_ptr + mlen + i)) XMSS_SIG_BYTES.
+
+print EncodeSignature. (* byte list -> sig_t *)
+print load_signature_mem. (* ptr & len  -> byte list *)
+
+lemma verify_correctness (mem : global_mem_t)  (ptr_m ptr_mlen ptr_sm sm_len : W64.t) (_pk : W8.t Array64.t) :
+    n = XMSS_N /\
+    d = XMSS_D /\
+    h = XMSS_FULL_HEIGHT =>
+    equiv [
+      M(Syscall).__xmssmt_core_sign_open ~ XMSS_MT_PRF.verify :
+      
+      Glob.mem{1} = mem /\
+
+      0 < to_uint (loadW64 mem (to_uint ptr_mlen)) < W64.max_uint /\
+      valid_ptr_i ptr_sm (4 + 32) /\
+
+      arg{1} = (ptr_m, ptr_mlen, ptr_sm, sm_len, _pk) /\
+      arg{2}.`1 = EncodePkNoOID _pk /\
+      arg{2}.`2 = load_sig_mem mem ptr_sm sm_len /\
+      arg{2}.`3 = EncodeSignature ( load_signature_mem mem ptr_sm (sm_len - W64.of_int XMSS_SIG_BYTES) )
+      ==>
+      res{2}  <=> res{1} = W64.zero /\
+      (!res{2} <=> res{1} = W64.of_int (-1))
+    ].
+proof.
+rewrite /XMSS_N /XMSS_D /XMSS_FULL_HEIGHT => [#] n_val d_val h_val.
+proc => /=. 
+seq 9 0 : #pre; first by auto.
+seq 29 17 : (is_valid{2} <=> are_equal{1} = W8.zero); last first.
+  + ecall {1} (p_set_result_post are_equal{1}).
+    auto => /> &1 r *.
+    case (are_equal{1} = W8.zero) => *.
+       - admit.
+       - admit.
+        
+seq 3 0 : (
+  #pre /\
+  sm_offset{1} = W64.zero /\
+  to_list pub_root{1} = sub pk{1} 0 32 /\
+  to_list pub_seed{1} = sub pk{1} 32 32
+).
+    + auto => /> *; do split.
+        * apply (eq_from_nth witness); first by rewrite size_to_list size_sub.
+          rewrite size_to_list => j?.
+          by rewrite nth_sub // get_to_list initiE. 
+        * apply (eq_from_nth witness); first by rewrite size_to_list size_sub.
+          rewrite size_to_list => j?.
+          by rewrite nth_sub // get_to_list initiE. 
+swap {1} 4 -2.
+seq 2 0 : (
+    #pre /\
+    ots_addr{1}.[0] = W32.zero /\
+    ots_addr{1}.[1] = W32.zero /\
+    ots_addr{1}.[2] = W32.zero /\
+    ots_addr{1}.[3] = W32.zero /\
+    ots_addr{1}.[4] = W32.zero /\
+    ots_addr{1}.[5] = W32.zero /\
+    ots_addr{1}.[6] = W32.zero /\
+    ots_addr{1}.[7] = W32.zero
+).
+    + inline M(Syscall).__zero_address_  M(Syscall).__set_type; wp; ecall {1} (zero_addr_res addr{1}).
+      auto => />.
+seq 4 0 : (
+    #pre /\
+    
+    ltree_addr{1}.[0] = W32.zero /\
+    ltree_addr{1}.[1] = W32.zero /\
+    ltree_addr{1}.[2] = W32.zero /\
+    ltree_addr{1}.[3] = W32.one /\
+    ltree_addr{1}.[4] = W32.zero /\
+    ltree_addr{1}.[5] = W32.zero /\
+    ltree_addr{1}.[6] = W32.zero /\
+    ltree_addr{1}.[7] = W32.zero /\
+  
+    node_addr{1}.[0] = W32.zero /\
+    node_addr{1}.[1] = W32.zero /\
+    node_addr{1}.[2] = W32.zero /\
+    node_addr{1}.[3] = W32.of_int 2 /\
+    node_addr{1}.[4] = W32.zero /\
+    node_addr{1}.[5] = W32.zero /\
+    node_addr{1}.[6] = W32.zero /\
+    node_addr{1}.[7] = W32.zero
+).
+    + inline {1} 3.
+      inline {1} 7. 
+      inline {1} 2.
+      wp.
+      ecall {1} (zero_addr_res addr1{1}).
+      inline {1} 1.
+      wp.
+      ecall {1} (zero_addr_res addr2{1}).
+      auto => />.
+ 
+(* this conseq simplifies #pre so that it fits on the screen *)
+conseq (:
+    Glob.mem{1} = mem /\
+    (0 < to_uint (loadW64 mem (to_uint ptr_mlen)) < W64.max_uint) /\
+    valid_ptr_i ptr_sm 36 /\
+    m_ptr{1} = ptr_m /\
+    mlen_ptr{1} = ptr_mlen /\
+    sm_ptr{1} = ptr_sm /\ 
+    smlen{1} = sm_len /\ 
+    pk{1} = _pk /\
+    pk{2} = EncodePkNoOID _pk /\
+    m{2} = load_sig_mem mem ptr_sm sm_len /\ 
+    s{2} = EncodeSignature
+       (load_signature_mem mem ptr_sm (sm_len - (of_int XMSS_SIG_BYTES)%W64)) /\
+    sm_offset{1} = W64.zero /\
+    to_list pub_root{1} = sub pk{1} 0 32 /\
+    to_list pub_seed{1} = sub pk{1} 32 32 /\
+
+    ots_addr{1} = zero_address /\
+    ltree_addr{1} = zero_address.[3 <- W32.one] /\
+    node_addr{1} = zero_address.[3 <- W32.of_int 2]
+
+    ==>
+    _
+).
+    + auto => /> &1 &2 *; do split.
+         * rewrite /zero_address tP => j?.
+           rewrite initiE // /#.
+         * rewrite /zero_address tP => j?.
+           rewrite get_setE // initiE //.
+           case (j = 3) => /#. 
+         * rewrite /zero_address tP => j?.
+           rewrite get_setE // initiE //.
+           case (j = 3) => /#. 
+
+(* This corresponds to *mlen = smlen - params->sig_bytes;
+   Not useful for the proof but #pre no longer holds 
+*)
+seq 3 0 : (
+  (0 < to_uint (loadW64 mem (to_uint ptr_mlen))  < W64.max_uint) /\
+  valid_ptr_i ptr_sm 36 /\
+  m_ptr{1} = ptr_m /\
+  mlen_ptr{1} = ptr_mlen /\
+  sm_ptr{1} = ptr_sm /\
+  smlen{1} = sm_len /\
+  pk{1} = _pk /\
+  pk{2} = EncodePkNoOID _pk /\
+  m{2} = load_sig_mem mem ptr_sm sm_len /\
+    s{2} = EncodeSignature
+       (load_signature_mem mem ptr_sm (sm_len - (of_int XMSS_SIG_BYTES)%W64)) /\
+  sm_offset{1} = W64.zero /\
+  to_list pub_root{1} = sub pk{1} 0 32 /\
+  to_list pub_seed{1} = sub pk{1} 32 32 /\
+  ots_addr{1} = zero_address /\
+  ltree_addr{1} = zero_address.[3 <- W32.one] /\
+  node_addr{1} = zero_address.[3 <- (of_int 2)%W32]
+); first by auto.
+
+seq 1 2 : (
+  #pre /\ 
+  to_uint idx{1} = to_uint idx_sig{2} /\
+  idx_sig{2} = s{2}.`sig_idx
+).
+    + auto => />.
+      admit. 
+
+(* This corresponds to the comment 
+
+    /* Put the message all the way at the end of the m buffer, so that we can
+     * prepend the required other inputs for the hash function. */      
+    
+    This is not useful for the proof 
+*)
+seq 4 0 : (#pre).
+    + seq 3 0 : (#pre /\ 0 <= to_uint bytes{1} < W64.max_uint).
+         * auto => /> &1 *; split. 
+              - admit.
+              - admit. (* A partir de #pre nao sei que Glob.mem.[ptr_m] = mem.[ptr_m] *)
+
+      inline {1}.
+      while {1} (#post) (to_uint bytes2{1} - to_uint i0{1}).
+         * auto => /> &hr *; smt(@W64 pow2_64).
+         * auto => /> &1 *; rewrite ultE /#.
+  
+seq 0 2 : (
+    #pre /\
+    val seed{2} = to_list pub_seed{1} /\
+    address{2} = zero_address
+).
+    + auto => /> &1 &2 ???? -> *. 
+      (* A seta refere se a hipotese to_list pub_seed{1} = sub _pk 32 32 *)
+      apply (eq_from_nth witness); first by rewrite valP n_val size_sub.
+      rewrite valP n_val => j?.
+      rewrite /EncodePkNoOID => />.
+      by rewrite insubdK; [by rewrite /P size_sub // n_val |].
+
+seq 3 0 : (
+  #pre /\
+  to_list buf{1} = mkseq (fun i => loadW8 Glob.mem{1} (to_uint sm_ptr{1} + 4 + i)) 32
+).
+    + ecall {1} (p_memcpy_ptr_correct t64{1}).
+      auto => /> &1 &2 *; do split. 
+         * rewrite to_uintD of_uintK /= /#.
+         * move => ?; rewrite to_uintD of_uintK /= /#. 
+         * rewrite to_uintD of_uintK /= /#.
+         * move => *.
+           apply (eq_from_nth witness); first by rewrite size_to_list size_mkseq. 
+           rewrite size_to_list => j?.
+           rewrite get_to_list initiE // nth_mkseq // => />.
+           congr. 
+           rewrite to_uintD_small 2:of_uintK // of_uintK /= /#.  
+
+swap {2} 5 -4.
+seq 0 1 : (#pre /\ to_list buf{1} = val _R{2}).
+    + auto => /> &1 &2 ???????? ->. 
+      apply (eq_from_nth witness).
+         * by rewrite valP n_val size_mkseq.
+      rewrite size_mkseq => j?.
+      rewrite /EncodeSignature => />.
+      rewrite insubdK; [by rewrite /P size_sub_list // n_val |].
+      rewrite /sub_list !nth_mkseq // => />.
+      rewrite /load_signature_mem nth_mkseq /XMSS_SIG_BYTES 1:/# => />.
+      rewrite to_uintD.
+      admit.
+
+
+seq 3 0  : (
+  #pre /\
+  to_uint t64{1} = to_uint m_ptr{1} + 2500 - 32 - 3*32 /\
+  to_uint bytes{1} = to_uint smlen{1} - XMSS_SIG_BYTES
+).
+    + auto => /> &1 &2 *; split.
+        * rewrite to_uintD of_uintK /=.  admit. (* Add info to precondition *)
+        * admit. (* Not enough info => Adicionar aquela parte que passei a frente *)
+
+seq 0 2 : (
+  #pre /\
+  idx_tree{2} = idx_sig{2} `>>>` 10 /\
+  idx_leaf{2} = idx_sig{2} `&` W32.of_int (2^10 - 1)
+); first by auto => /> &1 &2 *; rewrite h_val d_val /=.
+
+swap {2} 2 -1.
+seq 0 1 : (#pre /\ val root{2} = sub pk{1} 0 32).
+    + auto => /> &1 &2 *.
+      apply (eq_from_nth witness).
+         * by rewrite valP n_val size_sub.
+      rewrite valP n_val => j?.
+      rewrite /EncodePkNoOID => />.
+      by rewrite insubdK // /P size_sub // n_val.
+
+swap {2} 1 4.
+
+seq 1 2 : (#pre /\ to_list root{1} = val _M'{2}).
+    + admit.
+
+
+seq 0 2 : (
+  0 < to_uint (loadW64 mem (to_uint ptr_mlen)) < W64.max_uint /\
+  valid_ptr_i ptr_sm 36 /\
+  m_ptr{1} = ptr_m /\
+  mlen_ptr{1} = ptr_mlen /\
+  sm_ptr{1} = ptr_sm /\
+  smlen{1} = sm_len /\
+  pk{1} = _pk /\
+  pk{2} = EncodePkNoOID _pk /\
+  m{2} = load_sig_mem mem ptr_sm sm_len /\
+  s{2} =
+    EncodeSignature (load_signature_mem mem ptr_sm  (sm_len - (of_int XMSS_SIG_BYTES)%W64)) /\
+  sm_offset{1} = W64.zero /\
+  to_list pub_root{1} = sub pk{1} 0 32 /\
+  to_list pub_seed{1} = sub pk{1} 32 32 /\
+  ots_addr{1} = zero_address /\
+  ltree_addr{1} = zero_address.[3 <- W32.one] /\
+  node_addr{1} = zero_address.[3 <- (of_int 2)%W32] /\
+  to_uint idx{1} = to_uint idx_sig{2} /\ idx_sig{2} = s{2}.`sig_idx /\
+  val seed{2} = to_list pub_seed{1}  /\
+  to_list buf{1} =
+    mkseq (fun (i0 : int) => loadW8 Glob.mem{1} (to_uint sm_ptr{1} + 4 + i0)) 32 /\
+  to_list buf{1} = val _R{2} /\
+  to_uint bytes{1} = to_uint smlen{1} - XMSS_SIG_BYTES /\
+  idx_tree{2} = idx_sig{2} `>>>` 10 /\
+  idx_leaf{2} = idx_sig{2} `&` (of_int (2 ^ 10 - 1))%W32 /\
+  val root{2} = sub pk{1} 0 32 /\
+  to_list root{1} = val _M'{2} /\
+  
+  
+  address{2} = zero_address.[1 <- idx_tree{2}]
+).
+    + auto => /> &1 &2 *.
+      rewrite /set_tree_addr /set_layer_addr.
+      rewrite tP => j?.
+      case (j = 0) => *. 
+         * by rewrite get_setE // ifF 1:/# get_setE // ifF 1:/# get_setE // ifT // get_setE // ifF 1:/# zero_addr_i.
+      case (j = 1) => *.
+         * rewrite get_setE // ifF 1:/# get_setE // ifT // get_setE // ifT //.
+           admit.
+     admit.
+
+
+seq 2 0 : (
+  0 < to_uint (loadW64 mem (to_uint ptr_mlen)) < W64.max_uint /\
+  valid_ptr_i ptr_sm 36 /\
+  m_ptr{1} = ptr_m /\
+  mlen_ptr{1} = ptr_mlen /\
+  sm_ptr{1} = ptr_sm /\
+  smlen{1} = sm_len /\
+  pk{1} = _pk /\
+  pk{2} = EncodePkNoOID _pk /\
+  m{2} = load_sig_mem mem ptr_sm sm_len /\
+  s{2} =
+    EncodeSignature (load_signature_mem mem ptr_sm  (sm_len - (of_int XMSS_SIG_BYTES)%W64)) /\
+  to_list pub_root{1} = sub pk{1} 0 32 /\
+  to_list pub_seed{1} = sub pk{1} 32 32 /\
+  ots_addr{1} = zero_address /\
+  ltree_addr{1} = zero_address.[3 <- W32.one] /\
+  node_addr{1} = zero_address.[3 <- (of_int 2)%W32] /\
+  to_uint idx{1} = to_uint idx_sig{2} /\ idx_sig{2} = s{2}.`sig_idx /\
+  val seed{2} = to_list pub_seed{1}  /\
+  to_list buf{1} =
+    mkseq (fun (i0 : int) => loadW8 Glob.mem{1} (to_uint sm_ptr{1} + 4 + i0)) 32 /\
+  to_list buf{1} = val _R{2} /\
+  to_uint bytes{1} = to_uint smlen{1} - XMSS_SIG_BYTES /\
+  idx_tree{2} = idx_sig{2} `>>>` 10 /\
+  idx_leaf{2} = idx_sig{2} `&` (of_int (2 ^ 10 - 1))%W32 /\
+  val root{2} = sub pk{1} 0 32 /\
+  to_list root{1} = val _M'{2} /\
+  
+  
+  address{2} = zero_address.[1 <- idx_tree{2}] /\
+
+  to_uint t64{1} = 36 /\ 
+  to_uint sm_offset{1} = 36
+); first by auto.
+
+
+(* Unroll the first iteration on the left hand side *)
+unroll {1} 2.
+
+(* inline {2} RootFromSig.rootFromSig. *)
+(* Outline the inner loop *)
+(* cf. https://github.com/EasyCrypt/easycrypt/wiki/%5BTactic%5D-Outline *)
+
+rcondt {1} 2; first by auto.
+
+seq 2 0 : (#pre /\ to_uint idx_leaf{1} = 2^10 - 1); first by auto.
+
+
+qed.
+
+
+
+(*
+(* We have that sub sm_ptr 0 4 = W32ofBytes x.sig_idx => TODO: I need to write this lemma *)
+    + admit.
+
+
+swap {2} [2..3] -1.
+seq 0 2 : (#pre /\ to_list pub_seed{1} = val seed{2}).
+    + auto => /> &1 &2 ???? H*.
+      apply (eq_from_nth witness); first by rewrite valP n_val size_to_list.
+      rewrite size_to_list => j?.
+      rewrite /EncodePkNoOID => />. 
+      rewrite insubdK; first by rewrite /P size_sub // n_val. 
+      by rewrite -get_to_list H.
+
+(* This corresponds to memcpy(m + params->sig_bytes, sm + params->sig_bytes, *mlen)
+   Lines  452 - 456 in the xmss_commons.jtmpl 
+*)
+seq 4 0 : (#pre).  (* this is irrelevant for the result of the proof => just stores *)
+    + admit.
+
+
+(* this conseq simplifies #pre so it fits on the screen *)
+conseq (:
+    Glob.mem{2} = mem /\
+  (0 < to_uint (loadW64 Glob.mem{1} (to_uint ptr_mlen))  < W64.max_uint) /\
+    mem_dif Glob.mem{1} Glob.mem{2} [to_uint mlen_ptr{1}] /\
+    t64{1} = smlen{1} - (of_int XMSS_SIG_BYTES)%W64 /\
+    m_ptr{1} = ptr_m /\
+    mlen_ptr{1} = ptr_mlen /\
+    sm_ptr{1} = ptr_sm /\
+    smlen{1} = sm_len /\
+    pk{1} = _pk /\
+    pk{2} = EncodePkNoOID _pk /\
+    m{2} = load_sig_mem mem ptr_sm sm_len /\
+    s{2} = witness /\
+    sm_offset{1} = W64.zero /\
+    to_list pub_root{1} = sub pk{1} 0 32 /\
+    to_list pub_seed{1} = sub pk{1} 32 32 /\
+    
+    ots_addr{1} = zero_address /\
+    ltree_addr{1} = zero_address.[3 <- W32.one] /\
+    node_addr{1} = zero_address.[3 <- W32.of_int 2]
+  ==>
+  _
+).
+    + auto => /> &1 &2 *; do split.
+         * rewrite /zero_address tP => j?.
+           rewrite initiE // /#.
+         * rewrite /zero_address tP => j?.
+           rewrite get_setE // initiE //.
+           case (j = 3) => /#. 
+         * rewrite /zero_address tP => j?.
+           rewrite get_setE // initiE //.
+           case (j = 3) => /#. 
+
+(* This corresponds to the comment 
+1) First we need to copy the randomness from sm + params->index_bytes to buf
+*)
+swap {2} 6 -5.
+seq 3 1 : (
+  #pre /\ 
+  to_list buf{1} = val _R{2}
+).
+    + admit.
+
+(* Unroll the first iteration on the left hand side *)
+unroll {1} 9.
+
+
+admit.
+qed.
+*)
